Work towards more compute-friendly equations

examples/Crypto/Keccak/keccakScript.sml
@@ -97,6 +97,12 @@ Definition state_array_to_string_def:
     FLAT (GENLIST (Plane a) 5)
 End
 
+Theorem LENGTH_state_array_to_string[simp]:
+  LENGTH (state_array_to_string a) = 25 * a.w
+Proof
+  rw[state_array_to_string_def]
+QED
+
 Triviality GENLIST_AND_LENGTH:
   GENLIST (λx. x < n ∧ P x) n = GENLIST P n
 Proof
@@ -168,6 +174,12 @@ Proof
   rw[wf_state_array_def, theta_def, restrict_def] \\ rw[]
 QED
 
+Theorem theta_w[simp]:
+  (theta a).w = a.w
+Proof
+  rw[theta_def]
+QED
+
 Definition rho_xy_def[simp]:
   rho_xy 0 = (1, 0) ∧
   rho_xy (SUC t) =
@@ -201,6 +213,12 @@ Proof
   rw[wf_state_array_def, rho_def, restrict_def] \\ rw[]
 QED
 
+Theorem rho_w[simp]:
+  (rho a).w = a.w
+Proof
+  rw[rho_def]
+QED
+
 Definition pi_def:
   pi a =
   a with A updated_by (λf. restrict a.w $ λ(x, y, z).
@@ -211,6 +229,12 @@ Theorem wf_pi[simp]:
   wf_state_array a ⇒ wf_state_array (pi a)
 Proof
   rw[wf_state_array_def, pi_def, restrict_def] \\ rw[]
+QED
+
+Theorem pi_w[simp]:
+  (pi a).w = a.w
+Proof
+  rw[pi_def]
 QED
 
 Definition chi_def:
@@ -225,6 +249,12 @@ Theorem wf_chi[simp]:
   wf_state_array a ⇒ wf_state_array (chi a)
 Proof
   rw[wf_state_array_def, chi_def, restrict_def] \\ rw[]
+QED
+
+Theorem chi_w[simp]:
+  (chi a).w = a.w
+Proof
+  rw[chi_def]
 QED
 
 Definition rc_step_def:
@@ -266,6 +296,12 @@ Proof
   rw[wf_state_array_def, iota_def, restrict_def] \\ rw[]
 QED
 
+Theorem iota_w[simp]:
+  (iota a i).w = a.w
+Proof
+  rw[iota_def]
+QED
+
 Definition Rnd_def:
   Rnd a = iota (chi (pi (rho (theta a))))
 End
@@ -276,6 +312,12 @@ Proof
   rw[Rnd_def]
   \\ DEP_REWRITE_TAC[wf_iota]
   \\ rw[]
+QED
+
+Theorem Rnd_w[simp]:
+  (Rnd a i).w = a.w
+Proof
+  rw[Rnd_def]
 QED
 
 (* N.B. We assume here that the round index is always non-negative, which is not
@@ -343,5 +385,289 @@ End
 Definition SHA3_512_def:
   SHA3_512 M = Keccak 1024 (M ++ [F; T]) 512
 End
+
+(* compute-friendly versions and tests *)
+
+(* TODO: move *)
+Theorem LOG_POW:
+  1 < b ==> LOG b (b ** n) = n
+Proof
+  strip_tac
+  \\ irule logrootTheory.LOG_UNIQUE
+  \\ rw[EXP]
+QED
+
+(* TODO: move *)
+Theorem FUNPOW_COMPOSE:
+  !n x f g h.
+  (!m. m < n ==> h(g(FUNPOW f m x)) = FUNPOW f m x)
+  ==>
+  FUNPOW (g o f o h) n (g x) =
+  g (FUNPOW f n x)
+Proof
+  Induct \\ rw[]
+  \\ rw[FUNPOW_SUC]
+QED
+
+(* TODO: move *)
+Theorem FUNPOW_CONG:
+  !n x f g.
+  (!m. m < n ==> f (FUNPOW f m x) = g (FUNPOW f m x))
+  ==>
+  FUNPOW f n x = FUNPOW g n x
+Proof
+  Induct \\ rw[FUNPOW_SUC]
+  \\ AP_TERM_TAC \\ rw[]
+QED
+
+(* TODO: move *)
+Theorem FUNPOW_invariant:
+  !m x.
+  P x /\ (!x. P x ==> P (f x)) ==>
+  P (FUNPOW f m x)
+Proof
+  Induct \\ rw[FUNPOW_SUC]
+QED
+
+Triviality iota_some_elim:
+  (some j. j ≤ l ∧ z = 2 ** j - 1)
+  = if z = 2 ** LOG2 (SUC z) - 1 ∧ LOG2 (SUC z) ≤ l
+    then SOME (LOG2 (SUC z))
+    else NONE
+Proof
+  DEEP_INTRO_TAC some_intro \\
+  rw[ADD1, SUB_ADD, LOG_POW, LOG2_def]
+QED
+
+Triviality iota_case_cond:
+  (case (if b then SOME x else NONE) of NONE => y | SOME z => f z) =
+  if b then f x else y
+Proof
+  rw[]
+QED
+
+Theorem iota_compute = iota_def |>
+  SIMP_RULE (srw_ss()) [iota_some_elim, iota_case_cond];
+
+Definition tabulate_array_def:
+  tabulate_array a =
+  a with A := restrict a.w (λ(x, y, z).
+    EL (y * 5 * a.w + x * a.w + z) (state_array_to_string a))
+End
+
+Definition tabulate_string_def:
+  tabulate_string w s = <|
+    w := w
+  ; A := restrict w (λ(x, y, z). EL (y * 5 * w + x * w + z) s)
+  |>
+End
+
+Theorem wf_tabulate_string[simp]:
+  wf_state_array (tabulate_string w s)
+Proof
+  rw[wf_state_array_def, tabulate_string_def, restrict_def]
+  \\ rw[]
+QED
+
+Theorem tabulate_string_w[simp]:
+  (tabulate_string w s).w = w
+Proof
+  rw[tabulate_string_def]
+QED
+
+Theorem tabulate_id:
+  wf_state_array a ⇒
+  tabulate_array a = a
+Proof
+  rw[wf_state_array_def, tabulate_array_def, state_array_component_equality]
+  \\ rw[state_array_to_string_def, FUN_EQ_THM, FORALL_PROD, restrict_def]
+  \\ rename1`(x,y,z)`
+  \\ Cases_on`x < 5` \\ fs[]
+  \\ Cases_on`y < 5` \\ fs[]
+  \\ Cases_on`z < a.w` \\ fs[]
+  \\ fs[NUMERAL_LESS_THM, EL_APPEND_EQN] \\ rw[]
+  \\ fs[Plane_def, EL_APPEND_EQN] \\ fs[Lane_def]
+QED
+
+Definition Rnd_string_def:
+  Rnd_string w s i =
+  let θ = state_array_to_string $ theta $ tabulate_string w s in
+  let ρ = state_array_to_string $ rho $ tabulate_string w θ in
+  let π = state_array_to_string $ pi $ tabulate_string w ρ in
+  let χ = state_array_to_string $ chi $ tabulate_string w π in
+  let ι = iota $ tabulate_string w χ in
+  state_array_to_string $ ι i
+End
+
+Theorem LENGTH_Rnd_string[simp]:
+  LENGTH (Rnd_string w s i) = 25 * w
+Proof
+  rw[Rnd_string_def]
+QED
+
+Theorem tabulate_state_array_to_string:
+  wf_state_array a ∧ w = a.w
+  ⇒
+  tabulate_string w (state_array_to_string a) = a
+Proof
+  strip_tac
+  \\ first_assum (mp_then Any
+       (CONV_TAC o (RHS_CONV o (REWR_CONV o SYM)))
+       tabulate_id)
+  \\ rw[tabulate_array_def, tabulate_string_def, state_array_component_equality]
+QED
+
+Theorem Rnd_string_Rnd:
+  w = b2w (LENGTH s) ⇒
+  Rnd_string w s i =
+  state_array_to_string (Rnd (string_to_state_array s) i)
+Proof
+  rw[Rnd_string_def, Rnd_def]
+  \\ AP_TERM_TAC
+  \\ AP_THM_TAC
+  \\ AP_TERM_TAC
+  \\ DEP_REWRITE_TAC[tabulate_state_array_to_string, wf_chi]
+  \\ simp[]
+  \\ rpt AP_TERM_TAC
+  \\ rw[string_to_state_array_def,
+        state_array_component_equality,
+        tabulate_string_def]
+  \\ rw[restrict_def, FUN_EQ_THM, FORALL_PROD]
+  \\ rw[EQ_IMP_THM]
+  \\ fs[LEFT_ADD_DISTRIB]
+QED
+
+Theorem Rnd_Rnd_string:
+  wf_state_array a ∧ w = a.w
+  ⇒
+  Rnd a i =
+  string_to_state_array (Rnd_string w (state_array_to_string a) i)
+Proof
+  rw[Rnd_def, Rnd_string_def]
+  \\ DEP_REWRITE_TAC[state_array_to_string_to_state_array]
+  \\ simp[]
+  \\ AP_THM_TAC \\ AP_TERM_TAC
+  \\ DEP_REWRITE_TAC[tabulate_state_array_to_string]
+  \\ simp[]
+QED
+
+Theorem Keccak_p_tabulate:
+  LENGTH s = 25 * divisor ⇒
+  Keccak_p n s =
+  let w = b2w (LENGTH s) in
+  let l = w2l w in
+  let i0 = 12 + 2 * l - n in
+  let i1 = 12 + 2 * l - 1 in
+  FST (FUNPOW (λ(s,i). (Rnd_string w s i, SUC i)) (SUC i1 - i0) (s, i0))
+Proof
+  rw[Keccak_p_def, string_to_state_array_w, ADD1]
+  \\ qmatch_goalsub_abbrev_tac`2 * l`
+  \\ qmatch_goalsub_abbrev_tac`(s, i)`
+  \\ qmatch_goalsub_abbrev_tac`FUNPOW k m`
+  \\ qmatch_goalsub_abbrev_tac`Rnd_string w`
+  \\ qmatch_goalsub_abbrev_tac`FUNPOW f m (s,i)`
+  \\ qspecl_then[`m`,`(s,i)`,`f`,
+       `string_to_state_array ## I`,
+       `state_array_to_string ## I`]mp_tac FUNPOW_COMPOSE
+  \\ simp[Abbr`f`, o_DEF, LAMBDA_PROD, PAIR_MAP]
+  \\ qmatch_goalsub_abbrev_tac`FST (FUNPOW k m x)`
+  \\ qmatch_goalsub_abbrev_tac`FUNPOW d m x`
+  \\ `∀x. w = (FST x).w ∧ wf_state_array (FST x) ⇒ d x = k x`
+  by (
+    simp[Abbr`d`,Abbr`k`, FUN_EQ_THM, FORALL_PROD]
+    \\ rw[Rnd_Rnd_string] )
+  \\ `FUNPOW k m x = FUNPOW d m x`
+  by (
+    irule FUNPOW_CONG
+    \\ qx_gen_tac`z`
+    \\ strip_tac
+    \\ irule EQ_SYM
+    \\ first_x_assum irule
+    \\ conj_tac
+    \\ qho_match_abbrev_tac`P (FUNPOW k z x)`
+    \\ irule FUNPOW_invariant
+    \\ simp[Abbr`P`, Abbr`x`, Abbr`k`, FORALL_PROD]
+    \\ simp[string_to_state_array_w] )
+  \\ fs[]
+  \\ disch_then (fn th => DEP_REWRITE_TAC[th])
+  \\ simp[]
+  \\ rw[]
+  \\ DEP_REWRITE_TAC[GEN_ALL string_to_state_array_to_string]
+  \\ simp[]
+  \\ qexists_tac`divisor`
+  \\ qmatch_goalsub_abbrev_tac`FUNPOW p z q`
+  \\ qho_match_abbrev_tac`P (FUNPOW p z q)`
+  \\ irule FUNPOW_invariant
+  \\ simp[Abbr`P`, Abbr`q`, Abbr`p`, FORALL_PROD, Abbr`w`, b2w_def]
+QED
+
+(* WIP
+
+val cs = num_compset();
+val () = extend_compset [
+  Tys [``:state_array``],
+  Defs [
+    restrict_def,
+    b2w_def,
+    w2l_def,
+    string_to_state_array_def,
+    Lane_def,
+    Plane_def,
+    state_array_to_string_def,
+    tabulate_string_def,
+    Rnd_string_def,
+    theta_c_def,
+    theta_d_def,
+    theta_def,
+    rho_def (* TODO: remove LEAST *),
+    pi_def,
+    chi_def,
+    rc_step_def,
+    rc_def,
+    iota_compute,
+    Keccak_p_tabulate (* TODO: specialise to remove condition *),
+    chunks_def,
+    pad10s1_def,
+    sponge_def,
+    Keccak_def,
+    Keccak_256_def],
+  Extenders [
+    listSimps.list_rws,
+    rich_listSimps.add_rich_list_compset,
+    pairLib.add_pair_compset,
+    add_bit_compset,
+    pred_setLib.add_pred_set_compset,
+    add_combin_compset]
+ ] cs
+
+val thm = CBV_CONV cs ``Keccak_256 []``
+
+val ctm = ``512``
+val ftm = ``Keccak_p 24``
+val btm = ``1600``
+val padtm = ``pad10s1``
+val rtm = ``1600 - ^ctm``
+val Ntm = ``[]: bool list``
+val dtm = ``256``
+val Ptm = ``^Ntm ++ ^padtm ^rtm (LENGTH ^Ntm)``
+val ntm = ``LENGTH ^Ptm DIV ^rtm``
+val ctm = ``^btm - ^rtm``
+val Pistm =  ``chunks ^rtm ^Ptm``
+val S0tm = ``REPLICATE ^btm F``
+val Stm = ``FOLDL (λSi Pi. ^ftm (MAP2 (λx y. x ⇎ y) Si (Pi ⧺ REPLICATE ^ctm F))) ^S0tm ^Pistm``
+
+val chunksrw = CBV_CONV cs ``chunks 1088 (pad10s1 1088 0)``
+val step1 = (SIMP_CONV (srw_ss()) [REPLICATE_compute, chunksrw]) Stm
+val step1args = step1 |> concl |> rhs |> strip_comb |> #2
+val n1tm = step1args |> el 1
+val s1tm = step1args |> el 2
+val atm = ``string_to_state_array ^s1tm``
+val ltm = ``w2l ^atm.w``
+val i0tm = ``12 + 2 * ^ltm - ^n1tm``
+val i1tm = ``12 + 2 * ^ltm - 1``
+val step2tm = ``Rnd ^atm ^i0tm``
+val step2atm = ``theta ^atm``
+
+*)
 
 val _ = export_theory();
